bad commit message

Reflection/Experiments/IndexErasure.lean
@@ -11,36 +11,23 @@ open Tyₛ Tyₚ Varₛ Varₚ
 
 -- # Erasure
 
-
 def eTyₛ : Tyₛ.{u} -> Tyₛ.{u}
 | _ => U
-
-abbrev ETyₛA Aₛ := TyₛA (eTyₛ Aₛ) -- actually this is a constant `ETyₛA := Type _`
 
 /-- For example maps sort-ctx `[Vec : Nat -> U, ...]` into `[VecE : U, ...]`. -/
 def eConₛ : Conₛ.{u} -> Conₛ.{u}
 | ⬝      => ⬝
 | Γₛ ▹ _ => eConₛ Γₛ ▹ U
 
-abbrev EConₛA.{u, v} Γₛ := ConₛA.{u, v} (eConₛ Γₛ)
-
-abbrev EVarₛ (Γₛ : Conₛ) : Type _ := Varₛ (eConₛ Γₛ) U
-
 /-- This is a no-op, other than changing the type of the variable. -/
 def eVarₛ : Varₛ Γₛ Aₛ -> Varₛ (eConₛ Γₛ) U
 | .vz   => .vz
 | .vs v => .vs (eVarₛ v)
 
-abbrev ETmₛ (Γₛ : Conₛ) : Type _ := Tmₛ (eConₛ Γₛ) U
-
 /-- For example maps `Vec : Nat -> U ⊢ Vec 123 : U` into `VecE : U ⊢ VecE : U`. -/
 def eTmₛ : Tmₛ Γₛ Aₛ -> Tmₛ (eConₛ Γₛ) U
 | .var v              => .var (eVarₛ v)
 | .app (A := _Aₛ) t u => eTmₛ t
-
-abbrev ETmₛA.{u, v} (T : Tmₛ.{u} Γₛ Aₛ) (γₛE : EConₛA.{u, v} Γₛ) : Type _ := TmₛA.{u, v} (eTmₛ.{u} T) γₛE
-
-abbrev ETyₚ (Γₛ : Conₛ) : Type _ := Tyₚ (eConₛ Γₛ)
 
 /-- For example for `Vec.nil`, maps `Vec : Nat -> U ⊢ Vec 0` into `VecE : U ⊢ VecE`,
 and for `Vec.cons` maps `Vec : Nat -> U ⊢ (n:Nat) -> α -> Vec n -> Vec (n+1)`
@@ -50,25 +37,49 @@ def eTyₚ {Γₛ : Conₛ} : Tyₚ Γₛ -> Tyₚ (eConₛ Γₛ)
 | PPi   T    Rest => PPi T (fun t => eTyₚ (Rest t))
 | PFunc Self Rest => PFunc (eTmₛ Self) (eTyₚ Rest)
 
-abbrev ETyₚA (A : Tyₚ Γₛ) (γₛE : EConₛA Γₛ) : Type _ := TyₚA (eTyₚ A) γₛE
-
-abbrev EConₚ (Γₛ : Conₛ) : Type _ := Conₚ (eConₛ Γₛ)
 def eConₚ : Conₚ Γₛ -> Conₚ (eConₛ Γₛ)
 | ⬝ => ⬝
 | Γ ▹ A => (eConₚ Γ) ▹ (eTyₚ A)
 
-abbrev EConₚA (Γ : Conₚ Γₛ) (γₛE : EConₛA Γₛ) : Type _ := ConₚA (eConₚ Γ) γₛE
-
-abbrev EVarₚ (Γ : Conₚ Γₛ) (A : Tyₚ Γₛ) : Type _ := Varₚ (eConₚ Γ) (eTyₚ A)
 def eVarₚ : Varₚ Γ A -> Varₚ (eConₚ Γ) (eTyₚ A)
 | .vz => .vz
 | .vs v => .vs (eVarₚ v)
 
-abbrev ETmₚ (Γ : Conₚ Γₛ) (A : Tyₚ Γₛ) : Type _ := Tmₚ (eConₚ Γ) (eTyₚ A)
 def eTmₚ : Tmₚ.{u, v} Γ A -> Tmₚ.{u, v} (eConₚ Γ) (eTyₚ A)
 | .var v => .var (eVarₚ v)
 | .app (A := _A) t u => .app (eTmₚ t) u
 | .appr t u => .appr (eTmₚ t) (eTmₚ u)
+
+abbrev ETyₛA Aₛ := TyₛA (eTyₛ Aₛ) -- actually this is a constant `ETyₛA := Type _`
+abbrev EConₛA.{u, v} Γₛ := ConₛA.{u, v} (eConₛ Γₛ)
+abbrev EVarₛ (Γₛ : Conₛ) : Type _ := Varₛ (eConₛ Γₛ) U
+abbrev ETmₛ (Γₛ : Conₛ) : Type _ := Tmₛ (eConₛ Γₛ) U
+abbrev ETmₛA.{u, v} (T : Tmₛ.{u} Γₛ Aₛ) (γₛE : EConₛA.{u, v} Γₛ) : Type _ := TmₛA.{u, v} (eTmₛ.{u} T) γₛE
+abbrev mkETyₛ (Ωₛ : Conₛ) (Ωₚ : Conₚ Ωₛ) {Aₛ : Tyₛ} (t : Tmₛ Ωₛ Aₛ) : TyₛA.{u, u+1} U.{u} := mkTyₛ.{u, u} (eConₛ Ωₛ) (eConₚ Ωₚ) (eTmₛ t)
+abbrev mkEConₛ (Ωₛ : Conₛ) (Ωₚ : Conₚ Ωₛ) : EConₛA.{u, u+1} Ωₛ                 := mkConₛ.{u, u} (eConₛ Ωₛ) (eConₚ Ωₚ)
+
+abbrev ETyₚ (Γₛ : Conₛ) : Type _ := Tyₚ (eConₛ Γₛ)
+abbrev ETyₚA (A : Tyₚ Γₛ) (γₛE : EConₛA Γₛ) : Type _ := TyₚA (eTyₚ A) γₛE
+abbrev EConₚ (Γₛ : Conₛ) : Type _ := Conₚ (eConₛ Γₛ)
+abbrev EConₚA (Γ : Conₚ Γₛ) (γₛE : EConₛA Γₛ) : Type _ := ConₚA (eConₚ Γ) γₛE
+abbrev EVarₚ (Γ : Conₚ Γₛ) (A : Tyₚ Γₛ) : Type _ := Varₚ (eConₚ Γ) (eTyₚ A)
+abbrev ETmₚ (Γ : Conₚ Γₛ) (A : Tyₚ Γₛ) : Type _ := Tmₚ (eConₚ Γ) (eTyₚ A)
+abbrev mkETyₚ.{u} (Ωₛ : Conₛ) (Ωₚ : Conₚ Ωₛ) {Aₚ : Tyₚ Ωₛ} (t : Tmₚ Ωₚ Aₚ) : ETyₚA Aₚ (mkEConₛ Ωₛ Ωₚ) := mkTyₚ.{u, u} (eConₛ Ωₛ) (eConₚ Ωₚ) (eTmₚ t)
+abbrev mkEConₚ (Ωₛ : Conₛ) (Ωₚ : Conₚ Ωₛ) : EConₚA.{u, u+1} Ωₚ (mkEConₛ Ωₛ Ωₚ) := mkConₚ.{u, u} (eConₛ Ωₛ) (eConₚ Ωₚ)
+
+theorem mkEConₛ_coherent {t : Tmₛ Ωₛ Aₛ} : TmₛA (eTmₛ t) (mkEConₛ Ωₛ Ωₚ) = mkETyₛ Ωₛ Ωₚ t := by
+  rw [mkEConₛ, mkETyₛ, mkConₛ]
+  rw [mkConₛ_coherent]
+  induction t with
+  | var v =>
+    simp [eTmₛ, TmₛA_var, mkTyₛ]
+    induction v with
+    | vz => rfl
+    | vs v =>
+      simp only [eVarₛ, VarₛA]
+      rw [SubₛTm]
+      rw [SubₛVar_id]
+  | app t u ih => rw [eTmₛ, ih]
 
 
 
@@ -81,29 +92,29 @@ def gTyₛ : (Aₛ : Tyₛ.{u}) -> TyₛA.{u, u+1} (eTyₛ Aₛ) -> Tyₛ.{u+1}
 | U         , aₛE => SPi aₛE             (fun _ => U)
 | SPi T Rest, aₛE => SPi (ULift.{u+1} T) (fun t => gTyₛ (Rest t.down) aₛE)
 
-abbrev GTyₛA.{u, v} Aₛ aₛE := TyₛA.{u+1, v} (gTyₛ Aₛ aₛE)
-
 /-- For example maps sort-stx `[Vec : Nat -> U]` into `[VecG : Nat -> VecE -> U]`. -/
 def gConₛ : (Γₛ : Conₛ.{u}) -> (γₛE : ConₛA.{u, u+1} (eConₛ.{u} Γₛ)) -> Conₛ.{u+1}
 | ⬝      , ⟨⟩         => ⬝
-| Γₛ ▹ Aₛ, ⟨γₛE, aₛE⟩ => Conₛ.ext.{_} (gConₛ Γₛ γₛE) (gTyₛ.{u} Aₛ aₛE)
-
-abbrev GConₛA (Γₛ : Conₛ.{u}) (γₛE : EConₛA.{u, u+1} Γₛ) : Type _
-  := ConₛA.{u+1, u+1} (gConₛ.{u} Γₛ γₛE)
-
+| Γₛ ▹ Aₛ, ⟨γₛE, aₛE⟩ => Conₛ.ext (gConₛ Γₛ γₛE) (gTyₛ Aₛ aₛE)
 -- /-- VecG : Nat -> VecE -> Type -/
 -- example : gConₛ Vₛ ⟨⟨⟩, VecE⟩ = (⬝ ▹ SPi Nat fun _ => SPi VecE fun _ => U) := rfl
 
+example : gConₛ ⬝ ⟨⟩ = .nil := rfl
+example : gConₛ (Γₛ ▹ Aₛ) ⟨γ, a⟩ = (gConₛ Γₛ γ) ▹ (gTyₛ Aₛ a) := rfl
+
 /-- Given a variable `Vec:N->U ⊢ VAR(Vec) : N->U`, we return `VecG:N->VecE->U ⊢ VAR(VecG) : N->VecE->U`.
   The runtime de-brujin value of this variable doesn't change. So this is basically just a cast operator. -/
-def gVarₛ : {Γₛ : Conₛ} -> (γₛE : ConₛA.{u,u+1} (eConₛ Γₛ)) ->
+def gVarₛ : {Γₛ : Conₛ} -> (γₛE : EConₛA.{u, u+1} Γₛ) ->
   (v : Varₛ Γₛ Aₛ) ->
   Varₛ (gConₛ Γₛ γₛE) (gTyₛ Aₛ (VarₛA (eVarₛ v) γₛE))
-| _ ▹ _, _       , .vz   => .vz
+| Γₛ ▹ Aₛ, ⟨γₛE, bₛE⟩       , .vz   => by rw [gConₛ]; exact .vz
 | _ ▹ _, ⟨γₛE, _⟩, .vs v => .vs (gVarₛ γₛE v)
+--   Varₛ (gConₛ Γₛ (mkEConₛ Γₛ Γₚ)) (gTyₛ Aₛ (VarₛA (eVarₛ v) (mkEConₛ Γₛ Γₚ)))
+-- | Γₛₛ, _,  .vz   => .vz
+-- | Γₛ, Γₚ, .vs v => .vs (gVarₛ (mkEConₛ Γₛ Γₚ) v)
 
-abbrev GTmₛ (Γₛ : Conₛ) (Aₛ : Tyₛ) (γₛE : ConₛA.{u,u+1} (eConₛ Γₛ)) (tE : ETmₛ Γₛ) : Type (u+2)
-  := Tmₛ.{u+1} (gConₛ Γₛ γₛE) (gTyₛ Aₛ (TmₛA tE γₛE))
+#check eVarₛ
+#check eTmₛ
 
 /-- Given `Γₛ ⊢ Self a₁ a₂ a₃ : U` returns `guard(Γₛ) ⊢ SelfG a₁ a₂ a₃ : SelfE -> U`.
 
@@ -111,15 +122,10 @@ abbrev GTmₛ (Γₛ : Conₛ) (Aₛ : Tyₛ) (γₛE : ConₛA.{u,u+1} (eConₛ
   it could be `Even @ 123` or `Odd @ 123`.
   So the output term's type needs to depend on `t`.  -/
 def gTmₛ : {Γₛ : Conₛ} -> (γₛE : EConₛA.{u, u+1} Γₛ) ->
+  -- (t : Tmₛ Γₛ Aₛ) -> Tmₛ (gConₛ Γₛ γₛE) (gTyₛ Aₛ aₛE)
   (t : Tmₛ Γₛ Aₛ) -> Tmₛ (gConₛ Γₛ γₛE) (gTyₛ Aₛ (TmₛA (eTmₛ t) γₛE))
-| Γₛ, γₛE, .var v              => by rw [eTmₛ, TmₛA]; exact .var (gVarₛ γₛE v)
+| Γₛ, γₛE, .var v              => .var (gVarₛ γₛE v)
 | Γₛ, γₛE, .app (A := _Aₛ) t u => .app (gTmₛ γₛE t) (.up u)
-
-abbrev GTmₛA (T : Tmₛ Γₛ Aₛ) (γₛE : EConₛA.{u, u+1} Γₛ) (γₛG : GConₛA.{u} Γₛ γₛE)
-  : GTyₛA.{u, u+1} Aₛ (ETmₛA T γₛE)
-  := TmₛA (gTmₛ γₛE T) γₛG
-
-abbrev GTyₚ (Γₛ : Conₛ) (γₛE : EConₛA.{u,u+1} Γₛ) : Type (u+2) := Tyₚ (gConₛ Γₛ γₛE)
 
 /-- For example maps the `Vec.cons` ctor of type
 ```
@@ -138,8 +144,6 @@ def gTyₚ (γₛE : ConₛA.{u, u+1} (eConₛ Γₛ)) : (A : Tyₚ Γₛ) -> (a
       PFunc (.app (gTmₛ γₛE Self) e) <| -- SelfG e ->
         gTyₚ γₛE Rest (aE e)
 
-abbrev GTyₚA (A : Tyₚ Γₛ) (γₛE : EConₛA Γₛ) (γₛG : GConₛA Γₛ γₛE) (aE : TyₚA (eTyₚ A) γₛE) : Type _ := TyₚA (gTyₚ γₛE A aE) γₛG
-
 def gConₚ.{u} {Γₛ : Conₛ.{u}} (γₛE : ConₛA.{u, u+1} (eConₛ Γₛ))
   : (Γ : Conₚ.{u} Γₛ) ->
     (γE : ConₚA.{u, u+1} (eConₚ Γ) γₛE) ->
@@ -147,13 +151,10 @@ def gConₚ.{u} {Γₛ : Conₛ.{u}} (γₛE : ConₛA.{u, u+1} (eConₛ Γₛ))
 | ⬝, ⟨⟩ => ⬝
 | Γ ▹ A, ⟨γE, aE⟩ => gConₚ γₛE Γ γE ▹ gTyₚ γₛE A aE
 
-abbrev GConₚA (Γ : Conₚ Γₛ) (γₛE : EConₛA Γₛ) (γₛG : GConₛA Γₛ γₛE) (γₚE : ConₚA (eConₚ Γ) γₛE) : Type _
-  := ConₚA (gConₚ γₛE Γ γₚE) γₛG
-
 /-- Cast `"Vec.cons"` to `"VecG.cons"`, similar to `guardTmₚ`. -/
 def gVarₚ : {Γ : Conₚ Γₛ} -> (γₛE : ConₛA.{u,u+1} (eConₛ Γₛ)) -> (γE : ConₚA.{u,u+1} (eConₚ Γ) γₛE) ->
   (v : Varₚ Γ A) ->
-  Varₚ (gConₚ γₛE Γ γE) (gTyₚ γₛE A (TmₚA (.var <| eVarₚ v) γE))
+  Varₚ (gConₚ γₛE Γ γE) (gTyₚ γₛE A (VarₚA (eVarₚ v) γE))
 | _ ▹ _, _  ,       _, .vz   => .vz
 | _ ▹ _, γₛE, ⟨γE, _⟩, .vs v => .vs (gVarₚ γₛE γE v)
 
@@ -169,60 +170,74 @@ def gTmₚ (γₛE : ConₛA.{u,u+1} (eConₛ Γₛ)) (γE : ConₚA.{u,u+1} (eC
   let g := gTmₚ γₛE γE u
   .appr (.app (gTmₚ γₛE γE t) e) g
 
+set_option pp.universes true in
+abbrev GTyₛA.{u, v} (Aₛ : Tyₛ.{u}) (aₛE : TyₛA.{u, u + 1} (eTyₛ.{u} Aₛ)) : Type ((max (u + 1) v) + 1)
+  := TyₛA.{u+1, v} (gTyₛ Aₛ aₛE)
+
+abbrev GConₛA.{u, v} (Γₛ : Conₛ.{u}) (γₛE : EConₛA.{u, u+1} Γₛ) : Type ((max (u+1) v) + 1)
+  := ConₛA.{u+1, max (u+1) v} (gConₛ.{u} Γₛ γₛE)
+
+abbrev GTmₛ (Γₛ : Conₛ) (Aₛ : Tyₛ) (γₛE : EConₛA.{u,u+1} Γₛ) (aₛE : TyₛA (eTyₛ Aₛ)) : Type (u+2)
+  := Tmₛ.{u+1} (gConₛ Γₛ γₛE) (gTyₛ Aₛ aₛE)
+
+abbrev GTmₛA (T : Tmₛ Γₛ Aₛ) (γₛE : EConₛA.{u, u+1} Γₛ) (γₛG : GConₛA.{u, u+1} Γₛ γₛE) : GTyₛA Aₛ (ETmₛA T γₛE)
+  := TmₛA (gTmₛ γₛE T) γₛG
+
+abbrev GTyₚ (Γₛ : Conₛ) (γₛE : EConₛA.{u,u+1} Γₛ) : Type (u+2)
+  := Tyₚ (gConₛ Γₛ γₛE)
+
+abbrev GTyₚA (A : Tyₚ Γₛ) (γₛE : EConₛA Γₛ) (γₛG : GConₛA Γₛ γₛE) (aE : TyₚA (eTyₚ A) γₛE) : Type _
+  := TyₚA (gTyₚ γₛE A aE) γₛG
+
+abbrev GConₚA (Γ : Conₚ Γₛ) (γₛE : EConₛA Γₛ) (γₛG : GConₛA Γₛ γₛE) (γₚE : ConₚA (eConₚ Γ) γₛE) : Type _
+  := ConₚA (gConₚ γₛE Γ γₚE) γₛG
+
 abbrev GTmₚ (Γ : Conₚ Γₛ) (A : Tyₚ Γₛ) (γₛE : EConₛA.{u,u+1} Γₛ) (γₚE : EConₚA.{u,u+1} Γ γₛE) (tE : ETmₚ.{u, v} Γ A)
   : Type ((max (u+1) v) + 1)
   := Tmₚ.{u+1, v} (gConₚ γₛE Γ γₚE) (gTyₚ γₛE A (TmₚA tE γₚE))
 
--- section
--- open Example
--- #reduce gTmₚ (Γₛ := Vₛ) (Γ := V String) ⟨⟨⟩, VecE⟩ ⟨⟨⟨⟩, VecE.nil⟩, VecE.cons⟩ (.var .vz)
--- #reduce gTmₚ (Γₛ := Vₛ) (Γ := V String) ⟨⟨⟩, VecE⟩ ⟨⟨⟨⟩, VecE.nil⟩, VecE.cons⟩ (.var (.vs .vz))
--- #reduce gConₚ (Γₛ := Vₛ) ⟨⟨⟩, VecE⟩ (V String) ⟨⟨⟨⟩, VecE.nil⟩, VecE.cons⟩
--- end
+def mkGTyₛ (Ωₛ : Conₛ) (Ωₚ : Conₚ Ωₛ) {Aₛ : Tyₛ} (t : Tmₛ Ωₛ Aₛ) : TyₛA.{_, _} (gTyₛ Aₛ (mkETyₛ Ωₛ Ωₚ t))
+  := mkTyₛ
+    (gConₛ Ωₛ (mkEConₛ Ωₛ Ωₚ))
+    (gConₚ (mkEConₛ Ωₛ Ωₚ) Ωₚ (mkEConₚ Ωₛ Ωₚ))
+    (mkEConₛ_coherent ▸ gTmₛ (mkEConₛ Ωₛ Ωₚ) t) -- unhappy that we need a cast here...
+
+def mkGConₛ.{u} (Ωₛ : Conₛ) (Ωₚ : Conₚ Ωₛ) : ConₛA (gConₛ Ωₛ (mkEConₛ Ωₛ Ωₚ))
+  := mkConₛ.{u+1, u} (gConₛ Ωₛ (mkEConₛ Ωₛ Ωₚ)) (gConₚ (mkEConₛ Ωₛ Ωₚ) Ωₚ (mkEConₚ Ωₛ Ωₚ))
+
+def mkGTyₚ.{u} (Ωₛ : Conₛ) (Ωₚ : Conₚ Ωₛ) {Aₚ : Tyₚ Ωₛ} (t : Tmₚ Ωₚ Aₚ)
+  := mkTyₚ.{u+1, u}
+    (gConₛ Ωₛ (mkEConₛ Ωₛ Ωₚ))
+    (gConₚ (mkEConₛ Ωₛ Ωₚ) Ωₚ (mkEConₚ Ωₛ Ωₚ))
+    (gTmₚ (mkEConₛ Ωₛ Ωₚ) (mkEConₚ Ωₛ Ωₚ) t)
+
+def mkGConₚ.{u} (Ωₛ : Conₛ) (Ωₚ : Conₚ Ωₛ)
+  := mkConₚ.{u+1, u} (gConₛ Ωₛ (mkEConₛ Ωₛ Ωₚ)) (gConₚ (mkEConₛ Ωₛ Ωₚ) Ωₚ (mkEConₚ Ωₛ Ωₚ))
 
 /-
   # Lowering
+
+  ## Lowering Sorts
 -/
 
-@[instance] def IsSimpleTy.decide' (Aₛ : Tyₛ) : Decidable (Aₛ = U)
-  := match h : Aₛ with
-    | U => .isTrue (by cases h; rfl)
-    | SPi .. => .isFalse (by simp only [h, not_false_eq_true])
-@[instance] def IsSimple.decide' : (Γₛ : Conₛ) -> Decidable (Γₛ = eConₛ Γₛ)
-| ⬝ => .isTrue rfl
-| Γₛ ▹ Aₛ =>
-  match hAₛ : Aₛ with
-  | U =>
-    match decide' Γₛ with
-    | .isTrue p => by
-      rw [eConₛ]
-      rw [<- p]
-      exact .isTrue rfl
-    | .isFalse p => by
-      cases hAₛ
-      simp_all [eConₛ]
-      exact inferInstance
-  | SPi _ _ => .isFalse (by simp only [eConₛ, Conₛ.ext.injEq, and_false, not_false_eq_true])
-/-- If the type is already simple, we don't need to lower it. -/
-def IsSimpleTy (Aₛ : Tyₛ) : Prop := Aₛ = U
-/-- If the type is already simple, we don't need to lower it. -/
-def IsSimple (Γₛ : Conₛ) : Prop := Γₛ = eConₛ Γₛ
-@[instance] def IsSimpleTy.decide (Aₛ : Tyₛ) : Decidable (IsSimpleTy Aₛ) := by unfold IsSimpleTy; exact inferInstance
-@[instance] def IsSimple.decide (Γₛ : Conₛ) : Decidable (IsSimple Γₛ) := by unfold IsSimple; exact inferInstance
+-- abbrev LTyₛA (Aₛ : Tyₛ.{u})                          : Type (u+2) := (aₛE : ETyₛA.{u,u+1} Aₛ) × GTyₛA.{u,u} Aₛ aₛE
+-- abbrev LConₛA (Γₛ : Conₛ)                            : Type (u+2) := (γₛE : EConₛA.{u,u+1} Γₛ) × GConₛA.{u+1, u} Γₛ γₛE
+-- abbrev LTmₛ (Γₛ : Conₛ) (Aₛ : Tyₛ) (γₛE : EConₛA Γₛ) : Type (u+2) := (tE  : ETmₛ Γₛ)   × GTmₛ Γₛ Aₛ γₛE tE
+-- abbrev LTmₛA {Γₛ : Conₛ} (T : Tmₛ.{u} Γₛ U) (γₛL : LConₛA Γₛ) : Type (u+1) := -- make this `... -> Type (max (u+1) v)` some day.
+--   (e : ETmₛA T γₛL.fst) × GTmₛA T γₛL.fst γₛL.snd e
 
--- ## Lowering Sorts
+def mkLTyₛ' : (Aₛ : Tyₛ) -> (aₛE : ETyₛA.{u} Aₛ) -> GTyₛA.{u, u+2} Aₛ aₛE -> TyₛA.{u, u+2} Aₛ
+| U       , E, G => (e : E) × G e
+| SPi X Aₛ, E, G => fun (x : X) => mkLTyₛ' (Aₛ x) E (G (.up x))
 
-abbrev LTyₛA (Aₛ : Tyₛ.{u})                          : Type (u+2) := (aₛE : ETyₛA.{u,u+1} Aₛ) × GTyₛA.{u,u} Aₛ aₛE
-abbrev LConₛA (Γₛ : Conₛ)                            : Type (u+2) := (γₛE : EConₛA Γₛ) × GConₛA Γₛ γₛE
-abbrev LTmₛ (Γₛ : Conₛ) (Aₛ : Tyₛ) (γₛE : EConₛA Γₛ) : Type (u+2) := (tE  : ETmₛ Γₛ)   × GTmₛ Γₛ Aₛ γₛE tE
-abbrev LTmₛA {Γₛ : Conₛ} (T : Tmₛ.{u} Γₛ U) (γₛL : LConₛA Γₛ) : Type (u+1) := -- make this `... -> Type (max (u+1) v)` some day.
-  (e : ETmₛA T γₛL.fst) × GTmₛA T γₛL.fst γₛL.snd e
+/-- Exactly same signature as `mkTyₛ` (other than two more universes), except produces pair of E and G. -/
+def mkLTyₛ (Ωₛ : Conₛ) (Ωₚ : Conₚ Ωₛ) {Aₛ : Tyₛ} (t : Tmₛ Ωₛ Aₛ) : TyₛA.{u, u+2} Aₛ
+  := mkLTyₛ' Aₛ (mkETyₛ.{u} Ωₛ Ωₚ t) (mkGTyₛ.{u,u} Ωₛ Ωₚ t)
 
-def mkLTyₛ' : (Aₛ : Tyₛ) -> LTyₛA.{u} Aₛ -> TyₛA.{u, u+1} Aₛ
-| U       , ⟨E, G⟩ => (e : E) × G e
-| SPi X Aₛ, ⟨E, G⟩ => fun (x : X) => mkLTyₛ' (Aₛ x) ⟨E, G (.up x)⟩
+-- def mkLConₛ := hard to define...
 
-def mkLTyₛ {Aₛ : Tyₛ} : TyₛA.{u, u+1} Aₛ := mkLTyₛ' Aₛ ⟨mkTyₛ ⟩
+-- ## Lowering Points
+-- def mkLTyₚ (Ωₛ : Conₛ) (Ωₚ : Conₚ Ωₛ) {A : Tyₚ Ωₛ} (t : Tmₚ Ωₚ A) : TyₚA A (mkLConₛ ...) := ...
 
 namespace Example
   universe u v
@@ -238,109 +253,213 @@ namespace Example
   def Vₚ (A : Type u) : Conₚ Vₛ := (⬝ ▹ Vₚ_nil) ▹ @Vₚ_cons A
 
   -- E
-  def VₛE : Conₛ     := eConₛ Vₛ
-  def VₚE : Conₚ VₛE := eConₚ (Vₚ (ULift String))
-  def VₛEA : EConₛA.{u, u+1} Vₛ.{u}                   := mkConₛ.{u,u} VₛE VₚE
-  def VₚEA : EConₚA.{u, u+1} (Vₚ (ULift String)) VₛEA := mkConₚ.{u,u} VₛE VₚE
-  def VecE : ETyₛA.{u, u+1} (SPi (ULift Nat) (fun _ => U)) := mkTyₛ.{u,u} VₛE VₚE (.var .vz)
-  example : VₛEA = ⟨⟨⟩, VecE⟩ := rfl -- actually surprised this works by rfl
-  #reduce VₚEA
+  -- def VₛE : Conₛ     := eConₛ Vₛ
+  -- def VₚE : Conₚ VₛE := eConₚ (Vₚ (ULift String))
+  -- def VₛEA : EConₛA.{u, u+1} Vₛ.{u}                   := mkConₛ.{u,u} VₛE VₚE
+  -- def VₚEA : EConₚA.{u, u+1} (Vₚ (ULift String)) VₛEA := mkConₚ.{u,u} VₛE VₚE
+  -- def VecE : ETyₛA.{u, u+1} (SPi (ULift Nat) (fun _ => U)) := mkTyₛ.{u,u} VₛE VₚE (.var .vz)
+  def VecE : ETyₛA.{u, u+1} (SPi (ULift Nat) (fun _ => U)) := mkETyₛ.{u} Vₛ (Vₚ (ULift String)) (.var .vz)
+  def VecE.nil  := mkETyₚ Vₛ (Vₚ (ULift String)) (.var (.vs .vz))
+  def VecE.cons := mkETyₚ Vₛ (Vₚ (ULift String)) (.var .vz)
 
   -- G
-  def VₛG : Conₛ     := gConₛ.{u} Vₛ VₛEA
-  def VₚG : Conₚ VₛG := gConₚ VₛEA (Vₚ (ULift String)) VₚEA
-  def VₛGA : ConₛA.{u+1, u+2} VₛG      := mkConₛ.{u+1, u} VₛG VₚG
-  def VₚGA : ConₚA.{u+1, u+2} VₚG VₛGA := mkConₚ.{u+1, u} VₛG VₚG
-  def VecG := mkTyₛ.{u+1, u} VₛG VₚG (.var .vz)
-  example : VₛGA = ⟨⟨⟩, VecG⟩ := rfl
-  #reduce VₚGA
+  -- def VₛG : Conₛ     := gConₛ.{u} Vₛ VₛEA
+  -- def VₚG : Conₚ VₛG := gConₚ VₛEA (Vₚ (ULift String)) VₚEA
+  -- def VₛGA : ConₛA.{u+1, u+2} VₛG      := mkConₛ.{u+1, u} VₛG VₚG
+  -- def VₚGA : ConₚA.{u+1, u+2} VₚG VₛGA := mkConₚ.{u+1, u} VₛG VₚG
+  -- def VecG := mkTyₛ.{u+1, u} VₛG VₚG (.var .vz)
+  def VecG      := mkGTyₛ.{u, u} Vₛ (Vₚ (ULift String)) (.var .vz)
+  def VecG.nil  := mkGTyₚ Vₛ (Vₚ (ULift String)) (.var (.vs .vz))
+  def VecG.cons := mkGTyₚ Vₛ (Vₚ (ULift String)) (.var .vz)
 
   -- L
-  def VₛL : Conₛ
-  def VecL : Nat -> Type (u+2) := fun (n : Nat) => (e : VecE) × VecG (.up (.up n)) e
-  def asfsdaf : LTyₛA Aₛ := ⟨VecE, VecG⟩
-  #reduce mkLTyₛ' (SPi Nat fun _ => U) ⟨VecE, VecG⟩
+  def VecL' : TyₛA (SPi (ULift Nat) fun _ => U) := mkLTyₛ Vₛ (Vₚ (ULift String)) (.var .vz)
+  def VecL : Nat -> Type (u+2) := fun n => (e : VecE) × VecG (.up (.up n)) e
+  def VecL.nil : VecL 0 := ⟨.nil, .nil⟩
+  def VecL.cons : (n : Nat) -> String -> VecL n -> VecL (n+1)
+    := fun n x v => ⟨.cons (.up n) (.up x) v.fst, .cons (.up (.up n)) (.up (.up x)) v.fst v.snd⟩
+
+  #check Vec
+  def _Vec  : ULift Nat ->                  Type (u+1) := mkTyₛ.{u, u} Vₛ (Vₚ (ULift String)) (.var .vz)
+  def _VecE :                               Type (u+1) := mkETyₛ.{u}   Vₛ (Vₚ (ULift String)) (.var .vz)
+  def _VecG : ULift (ULift Nat) -> _VecE -> Type (u+2) := mkGTyₛ.{u, u}   Vₛ (Vₚ (ULift String)) (.var .vz)
+  def _VecL : Nat ->                        Type (u+2) := fun n => (e : VecE) × VecG (.up (.up n)) e
 end Example
 
-namespace Example
-  #reduce LTyₛA (SPi Nat fun _ => U)
-  #check mkLTyₛ (SPi Nat fun _ => U) ⟨VecE, VecG⟩
-  #reduce mkLTyₛ (SPi Nat fun _ => U) ⟨VecE, VecG⟩
-  #check @TyₛA
-  #check @LTyₛA
-end Example
+/-
+  ## Lowering Terms
+  This is done via good old Lean metaprogramming.
+-/
 
-/-- For example maps `"Vec 123"` to `⟨"VecE", "VecG 123"⟩`. -/
-def lTmₛ {Γₛ : Conₛ} {Aₛ : Tyₛ} (γₛE : ConₛA (eConₛ Γₛ)) (t : Tmₛ Γₛ Aₛ) : LTmₛ Γₛ Aₛ γₛE
-  := ⟨eTmₛ t, gTmₛ γₛE t⟩
+open Lean Elab Term Meta
+-- open Qq
 
-/-- We want to obtain the actual `(e : VecE) × VecG e`. -/
-def lTmₛA (γₛE : ConₛA (eConₛ Γₛ)) (γₛG : ConₛA (gConₛ Γₛ γₛE)) (T : Tmₛ Γₛ U) : Type _
-  := @Sigma (ETmₛA T γₛE) (GTmₛA T γₛE γₛG)
+def lowerDef (e : Expr) : MetaM Expr := do sorry
 
-#reduce lTmₛA ⟨⟨⟩, VecE⟩ ⟨⟨⟩, VecG⟩ (.var .vz)
+def lowerInduct (e : Expr) : MetaM Expr := do
+  let Γₛ : Expr := sorry
+  let Γₚ : Expr := sorry
 
-/-- Construct new inductive types. -/
-def lConₛA : (Γₛ : Conₛ) -> (Γₚ : Conₚ Γₛ) -> LConₛA.{0,0} Γₛ
-| Γₛ, Γₚ =>
-  let γₛE : EConₛA Γₛ     := mkConₛ (Ω := eConₚ Γₚ)
-  let γₛG : GConₛA Γₛ γₛE := mkConₛ (Ω := gConₚ γₛE Γₚ)
-  -- ⟨γₛE, γₛG⟩
-  sorry -- the above works, modulo universe shenanigans
+  sorry
+  -- let ΓₚE : Q(Conₚ $ΓₛE) := mkApp2 q(@eConₚ.{0}) Γₛ Γₚ
+  -- let γₛE : Q(EConₛA.{0,0} $Γₛ)      := mkApp2 q(@mkConₛ.{0}) ΓₛE ΓₚE
+  -- let γₚE : Q(EConₚA.{0,0} $Γₚ $γₛE) := mkApp2 q(@mkConₚ.{0}) ΓₛE ΓₚE
 
--- ## Lowering Points
+  -- let ΓₛG : Q(Conₛ.{0}) := mkApp2 q(@gConₛ.{0}) Γₛ γₛE
+  -- let ΓₚG : Q(Conₚ $ΓₛG) := mkApp4 q(@gConₚ) Γₛ γₛE Γₚ γₚE
+  -- let γₛG /- : Q(GConₛA.{0,0} ..) -/ := mkApp2 q(@mkConₛ.{0}) ΓₛG ΓₚG
+  -- let γₚG /- : Q(GConₚA.{0,0} ..)-/ := mkApp2 q(@mkConₚ.{0}) ΓₛG ΓₚG
+  -- -- let L : Q(Type) := q(@Sigma )
+-- #exit
 
-abbrev LTyₚA (A : Tyₚ Γₛ) (γₛL : LConₛA Γₛ) : Type _ := (e : ETyₚA A γₛL.fst) × GTyₚA A γₛL.fst γₛL.snd e
-abbrev LConₚA (Γ : Conₚ Γₛ) (γₛL : LConₛA Γₛ) : Type _ := (e : EConₚA Γ γₛL.fst) × GConₚA Γ γₛL.fst γₛL.snd e
-abbrev LTmₚ {Γₛ : Conₛ} (Γ : Conₚ Γₛ) (A : Tyₚ Γₛ) (γₛE) (γₚE : ConₚA (eConₚ Γ) γₛE) : Type _
-  := (tE : ETmₚ Γ A) × GTmₚ Γ A γₛE γₚE tE
+/-- Given `Vec 123`, produces `VecL 123`. -/
+def lowerTmₛ (e : Expr) : MetaM Expr := do
+  sorry
 
-/-- Given a term `"Vec.cons n x v"`, produce
-  `⟨"VecE.cons n x vᴱ", "VecG.cons n x vᴱ vᴳ"⟩ : Tmₛ ["VecE"] "U" × Tmₛ ["VecG"] "VecE -> U"`. -/
-def lTmₚ {Γₛ : Conₛ} {Γ : Conₚ Γₛ} {A : Tyₚ Γₛ} {γₛE} {γₚE : ConₚA (eConₚ Γ) γₛE}
-  (t : Tmₚ Γ A) : LTmₚ Γ A γₛE γₚE
-  := ⟨eTmₚ t, gTmₚ γₛE γₚE t⟩
+/-- Given `Vec.cons`, produces `VecL.cons`. -/
+def lowerTyₚ (e : Expr) : MetaM Expr := do
+  sorry
 
-/-- Given `"Vec.cons ..." : "Vec 123"`, produce `⟨VecE.cons ..., VecG.cons ...⟩ : @Sigma VecE (VecG 123)`. -/
-def lTmₚA (γₛE : ConₛA (eConₛ Γₛ)) (γₛG : ConₛA (gConₛ Γₛ γₛE))
-  (γE : ConₚA (eConₚ Γ) γₛE) (γG : ConₚA (gConₚ γₛE Γ γE) γₛG)
-  (t : Tmₚ Γ (El T))
-  : lTmₛA γₛE γₛG T
-  := by
-    let g := TmₚA (gTmₚ γₛE γE t) γG
-    rw [gTyₚ] at g
-    rw [TyₚA] at g
-    rw [TmₛA] at g
-    exact ⟨TmₚA (eTmₚ t) γE, g⟩
+/-- Lowers a term.  -/
+def lowerTm (e : Expr) : MetaM Expr := do
+  match e with
+  | .app f a =>
+    -- `⊢ f : Pi A B`
+    -- `⊢ a : A`
+    -- `f a : B[a]`
+    -- `⊢ fᴸ : Pi Aᴸ Bᴸ`
+    return .app (<- lowerTm f) (<- lowerTm a)
+  -- | .lam .. => sorry
+  | .const name _ =>
+    match <- getConstInfo name with
+    | .inductInfo _ => lowerInduct e
+    | .ctorInfo _ => lowerTyₚ e
+    | .defnInfo _ => lowerDef e
+    | _ => throwError "lowerEnv: unsupported const kind for {name}"
+  | _ => throwError "oh no, lowerTm {e}"
 
-section
-  open Example
-  -- Sorts
-  example : LConₛA Vₛ = ((γₛE : PUnit.{2} × Type) × (PUnit.{2} × (Nat → γₛE.snd → Type))) := rfl
-  example : LConₛA Vₛ := ⟨⟨⟨⟩, VecE⟩, ⟨⟨⟩, VecG⟩⟩
-  /-- `"Vec 123" : "U"` becomes `⟨"VecE", "VecG 123"⟩ : "U" × "VecE -> U"` -/
-  example : lTmₛ  (Γₛ := Vₛ) ⟨⟨⟩, VecE⟩            (.app (.var .vz) 123) = ⟨.var .vz, .app (.var .vz) 123⟩ := rfl
-  example : lTmₛA (Γₛ := Vₛ) ⟨⟨⟩, VecE⟩ ⟨⟨⟩, VecG⟩ (.app (.var .vz) 123) = @Sigma VecE (VecG 123)          := rfl
+/-- Lowers a type. `lower : Ty Γ -> Ty Γᴸ`
+```
+def lowerTy : {Γ : Con} -> Ty Γ -> Ty Γᴸ
+| Γ, .Pi A B => -- where `Ty.Pi : (A : Ty Γ) -> Ty (Γ, A) -> Ty Γ`
+  let AL : Ty Γᴸ := lowerTy A
+  let BL : Ty (Γᴸ, Aᴸ) := lowerTy B -- because `(Γ, A)ᴸ ≣ (Γᴸ, Aᴸ)`
+  .Pi AL BL -- typechecks
+| Γ, El T => sorry
+``` -/
+partial def lowerTy (u : Level) (e : Expr) : MetaM Expr := do
+  if let Expr.sort _ := e then -- case `U : Ty Γ`
+    return e
+  else if let .forallE _ A _ _ := e then -- case `Pi A B : Ty Γ`
+    Meta.forallBoundedTelescope e (some 1) fun a_fv B => do
+      let Γ_A <- getLCtx -- `Γ, A` and `Γ, A ⊢ B`
+      let AL : Expr <- lowerTy u A -- Γᴸ ⊢ Aᴸ
+      let BL : Expr <- lowerTy u B -- (Γ, A)ᴸ ⊢ Bᴸ    is (hopefully) well-typed again.
+      let Γ_AL := Γ_A.modifyLocalDecl a_fv[0]!.fvarId! (fun ldecl => ldecl.setType AL)
+      withLCtx Γ_AL (<- getLocalInstances) do
+        mkForallFVars a_fv BL
+  else if let .fvar fv := e then
+    -- `⊢ a : A` gets casted to `⊢ aL : Aᴸ`. Since metaprogramming is untyped, this is a no-op.
+    return .fvar fv
+  else -- case `El T : Ty Γ`
+    lowerTm e
+    -- let T := e.getAppFn
+    -- let args := e.getAppArgs
+    -- let v <- mkFreshLevelMVar
+    -- if <- isDefEq T (.const ``Vec [v]) then
+    --   let n := args[1]!
+    --   return mkAppN (.const ``Sigma [u, u]) #[.const ``Example.VecE [u], .app (.const ``Example.VecG [u]) n]
+    -- else if T.isAppOf ``Eq then return mkAppN (.const ``Eq [.zero]) args
+    -- else if T.isAppOf ``Nat || T.isAppOf ``String then return e
+    -- else throwError "oh no, {e}"
 
-  -- Points
-  example : lTmₚA (Γₛ := Vₛ) (Γ := V String)
-    ⟨⟨⟩, VecE⟩ ⟨⟨⟩, VecG⟩ ⟨⟨⟨⟩, VecE.nil⟩, VecE.cons⟩ ⟨⟨⟨⟩, VecG.nil⟩, VecG.cons⟩
-    (.var (.vs .vz))
-    = ⟨VecE.nil, VecG.nil⟩ := rfl
-  example : lTmₚA (Γₛ := Vₛ) (Γ := V String)
-    ⟨⟨⟩, VecE⟩                  ⟨⟨⟩, VecG⟩
-    ⟨⟨⟨⟩, VecE.nil⟩, VecE.cons⟩ ⟨⟨⟨⟩, VecG.nil⟩, VecG.cons⟩
-    (
-      let asdf1 : Tmₚ (V String) (PPi String fun _x => PFunc (.app (Tmₛ.var vz) 0) (El _)) := .app (.var .vz) 0
-      let asdf2 : Tmₚ (V String) (                     PFunc (.app (Tmₛ.var vz) 0) (El _)) := .app asdf1 "" -- ! if you inline `asdf1` it breaks
-      let asdf3 : Tmₚ (V String) (                                                 (El _)) := .appr asdf2 (.var (.vs .vz))
-      asdf3 -- ! if you inline asdf3 is breaks as well
-    )
-    = ⟨VecE.cons 0 "" VecE.nil, VecG.cons 0 "" VecE.nil VecG.nil⟩
-    := rfl
-end
+-- open Example
+@[irreducible] def len  : Vec String n -> Nat := fun _ => n
+
+elab "lower! " T:term : term => do
+  let T <- elabTerm T none
+  let u <- Meta.mkFreshLevelMVar
+  lowerTy (u := u) T
+
+#check ∀n, ∀x, lower! ∀v, len (Vec.cons n x v) = (len v) + 1
+/- (n : Nat) → (x : String) → (v : PSigma (VecG n)) → TEq (len (Vec.cons n x v)) (len v + 1) -/
+
+-- #eval lowerTy q((v : MutualInductive.Vec String (nat_lit 0)) -> TEq (len (Vec.cons 0 "a" v)) ((len v) + 1))
+
+
 
 #exit
+
+-- /-- For example maps `"Vec 123"` to `⟨"VecE", "VecG 123"⟩`. -/
+-- def lTmₛ {Γₛ : Conₛ} {Aₛ : Tyₛ} (γₛE : ConₛA (eConₛ Γₛ)) (t : Tmₛ Γₛ Aₛ) : LTmₛ Γₛ Aₛ γₛE
+--   := ⟨eTmₛ t, gTmₛ γₛE t⟩
+
+-- /-- We want to obtain the actual `(e : VecE) × VecG e`. -/
+-- def lTmₛA (γₛE : ConₛA (eConₛ Γₛ)) (γₛG : ConₛA (gConₛ Γₛ γₛE)) (T : Tmₛ Γₛ U) : Type _
+--   := @Sigma (ETmₛA T γₛE) (GTmₛA T γₛE γₛG)
+
+
+-- /-- Construct new inductive types. -/
+-- def mkLConₛ : (Γₛ : Conₛ) -> (Γₚ : Conₚ Γₛ) -> ConₛA.{0,0} Γₛ
+-- | Γₛ, Γₚ =>
+--   let γₛE := mkEConₛ Γₛ Γₚ
+--   let γₛG := mkGConₛ Γₛ Γₚ
+--   @Sigma γₛE
+
+
+-- abbrev LTyₚA (A : Tyₚ Γₛ) (γₛL : LConₛA Γₛ) : Type _ := (e : ETyₚA A γₛL.fst) × GTyₚA A γₛL.fst γₛL.snd e
+-- abbrev LConₚA (Γ : Conₚ Γₛ) (γₛL : LConₛA Γₛ) : Type _ := (e : EConₚA Γ γₛL.fst) × GConₚA Γ γₛL.fst γₛL.snd e
+-- abbrev LTmₚ {Γₛ : Conₛ} (Γ : Conₚ Γₛ) (A : Tyₚ Γₛ) (γₛE) (γₚE : ConₚA (eConₚ Γ) γₛE) : Type _
+--   := (tE : ETmₚ Γ A) × GTmₚ Γ A γₛE γₚE tE
+
+-- /-- Given a term `"Vec.cons n x v"`, produce
+--   `⟨"VecE.cons n x vᴱ", "VecG.cons n x vᴱ vᴳ"⟩ : Tmₛ ["VecE"] "U" × Tmₛ ["VecG"] "VecE -> U"`. -/
+-- def lTmₚ {Γₛ : Conₛ} {Γ : Conₚ Γₛ} {A : Tyₚ Γₛ} {γₛE} {γₚE : ConₚA (eConₚ Γ) γₛE}
+--   (t : Tmₚ Γ A) : LTmₚ Γ A γₛE γₚE
+--   := ⟨eTmₚ t, gTmₚ γₛE γₚE t⟩
+
+-- /-- Given `"Vec.cons ..." : "Vec 123"`, produce `⟨VecE.cons ..., VecG.cons ...⟩ : @Sigma VecE (VecG 123)`. -/
+-- def lTmₚA (γₛE : ConₛA (eConₛ Γₛ)) (γₛG : ConₛA (gConₛ Γₛ γₛE))
+--   (γE : ConₚA (eConₚ Γ) γₛE) (γG : ConₚA (gConₚ γₛE Γ γE) γₛG)
+--   (t : Tmₚ Γ (El T))
+--   : lTmₛA γₛE γₛG T
+--   := by
+--     let g := TmₚA (gTmₚ γₛE γE t) γG
+--     rw [gTyₚ] at g
+--     rw [TyₚA] at g
+--     rw [TmₛA] at g
+--     exact ⟨TmₚA (eTmₚ t) γE, g⟩
+
+-- section
+--   open Example
+--   -- Sorts
+--   example : LConₛA Vₛ = ((γₛE : PUnit.{2} × Type) × (PUnit.{2} × (Nat → γₛE.snd → Type))) := rfl
+--   example : LConₛA Vₛ := ⟨⟨⟨⟩, VecE⟩, ⟨⟨⟩, VecG⟩⟩
+--   /-- `"Vec 123" : "U"` becomes `⟨"VecE", "VecG 123"⟩ : "U" × "VecE -> U"` -/
+--   example : lTmₛ  (Γₛ := Vₛ) ⟨⟨⟩, VecE⟩            (.app (.var .vz) 123) = ⟨.var .vz, .app (.var .vz) 123⟩ := rfl
+--   example : lTmₛA (Γₛ := Vₛ) ⟨⟨⟩, VecE⟩ ⟨⟨⟩, VecG⟩ (.app (.var .vz) 123) = @Sigma VecE (VecG 123)          := rfl
+
+--   -- Points
+--   example : lTmₚA (Γₛ := Vₛ) (Γ := V String)
+--     ⟨⟨⟩, VecE⟩ ⟨⟨⟩, VecG⟩ ⟨⟨⟨⟩, VecE.nil⟩, VecE.cons⟩ ⟨⟨⟨⟩, VecG.nil⟩, VecG.cons⟩
+--     (.var (.vs .vz))
+--     = ⟨VecE.nil, VecG.nil⟩ := rfl
+--   example : lTmₚA (Γₛ := Vₛ) (Γ := V String)
+--     ⟨⟨⟩, VecE⟩                  ⟨⟨⟩, VecG⟩
+--     ⟨⟨⟨⟩, VecE.nil⟩, VecE.cons⟩ ⟨⟨⟨⟩, VecG.nil⟩, VecG.cons⟩
+--     (
+--       let asdf1 : Tmₚ (V String) (PPi String fun _x => PFunc (.app (Tmₛ.var vz) 0) (El _)) := .app (.var .vz) 0
+--       let asdf2 : Tmₚ (V String) (                     PFunc (.app (Tmₛ.var vz) 0) (El _)) := .app asdf1 "" -- ! if you inline `asdf1` it breaks
+--       let asdf3 : Tmₚ (V String) (                                                 (El _)) := .appr asdf2 (.var (.vs .vz))
+--       asdf3 -- ! if you inline asdf3 is breaks as well
+--     )
+--     = ⟨VecE.cons 0 "" VecE.nil, VecG.cons 0 "" VecE.nil VecG.nil⟩
+--     := rfl
+-- end
+
+
+
+-- #exit
 
 /- # Reconstruction for Mutually Inductive Types
   Given `P : Vec n -> Prop`, We can derive `P' : @Sigma VecE (VecG n) -> Prop`.
@@ -351,17 +470,14 @@ end
   We derive `P' : Sigma VecE (VecG n) -> Prop`, such that `P' (down v) -> P v`. !!! how "such that"? This is the crucial part.
 -/
 
--- This is just `rTyₛA {Aₛ} _ ≣ TyₛA Aₛ` ?
-def rTyₛA : {Aₛ : Tyₛ} -> LTyₛA.{0,0,0} Aₛ -> TyₛA Aₛ
-| U      , _      => Type
-| SPi X _, ⟨E, G⟩ => fun (x : X) => rTyₛA ⟨E, G x⟩
+-- -- This is just `rTyₛA {Aₛ} _ ≣ TyₛA Aₛ` ?
+-- def rTyₛA : {Aₛ : Tyₛ} -> LTyₛA.{0,0,0} Aₛ -> TyₛA Aₛ
+-- | U      , _      => Type
+-- | SPi X _, ⟨E, G⟩ => fun (x : X) => rTyₛA ⟨E, G x⟩
 
-def rConₛA : {Γₛ : Conₛ} -> LConₛA Γₛ -> ConₛA Γₛ
-| ⬝    , ⟨⟨⟩, ⟨⟩⟩ => ⟨⟩
-| _ ▹ _, ⟨⟨γE, aE⟩, ⟨γG, aG⟩⟩ => ⟨rConₛA ⟨γE, γG⟩, rTyₛA ⟨aE, aG⟩⟩
-
--- * I think the idea should be to provide an eliminator for L, which is exactly as powerful
--- * as the original eliminator.
+-- def rConₛA : {Γₛ : Conₛ} -> LConₛA Γₛ -> ConₛA Γₛ
+-- | ⬝    , ⟨⟨⟩, ⟨⟩⟩ => ⟨⟩
+-- | _ ▹ _, ⟨⟨γE, aE⟩, ⟨γG, aG⟩⟩ => ⟨rConₛA ⟨γE, γG⟩, rTyₛA ⟨aE, aG⟩⟩
 
 def rTyₛD : (Aₛ : Tyₛ) -> (aₛL : LTyₛA Aₛ) -> (eD : TyₛD (eTyₛ Aₛ) aₛL.fst) × TyₛD (gTyₛ Aₛ aₛL.fst) aₛL.snd
 | U       , τ => sorry
@@ -393,22 +509,18 @@ def rTyₚA : {A : Tyₚ Γₛ} -> LTyₚA A γₛL -> TyₚA A γₛ
 def rConₚA : {Γ : Conₚ Γₛ} -> LConₚA Γ γₛL -> ConₚA Γ γₛ
 | Γ, γₚL => sorry
 
-namespace Example
-  def VecL (n) := @Sigma VecE (VecG n)
-  def nilL : VecL 0 := ⟨.nil, .nil⟩
-  def consL : (n : Nat) -> String -> VecL n -> VecL (n + 1)
-    := fun n x v => ⟨.cons n x v.fst, .cons n x v.fst v.snd⟩
 
+namespace Example
   set_option linter.unusedVariables false in
   /-- You can specify an eliminator for VecL, which behaves exactly the way that Vec.rec does. -/
   noncomputable def VecL.elim
     {motive : (n : Nat) -> VecL n -> Sort u}
     (nilD : motive 0 nilL)
-    (consD : (n : Nat) -> (x : String) -> (vL : VecL n) -> motive n vL -> motive (n + 1) (consL n x vL))
+    (consD : (n : Nat) -> (x : String) -> (vL : VecL n) -> motive n vL -> motive (n + 1) (.cons n x vL))
     (n : Nat)
     (vL : VecL n)
     : motive n vL :=
-    @VecE.rec (fun vE => (vG : VecG n vE) -> motive n ⟨vE, vG⟩)
+    VecE.rec (fun vE => (vG : VecG n vE) -> motive n ⟨vE, vG⟩)
       (fun vG =>
         @VecG.rec (fun n vE vG => motive n ⟨vE, vG⟩)
           nilD
@@ -476,7 +588,7 @@ namespace Example
 end Example
 
 
-
+#exit
 
 /-
   # Reconstruction for whole Formulas
@@ -521,23 +633,6 @@ abbrev Ty (_Γ : LocalContext) : Type := Q(Type)
 abbrev lowerCon : LocalContext -> LocalContext := id
 
 def lowerEnvDef (e : Expr) : MetaM Expr := do sorry
-
--- mk
-#check @mkConₛ
-#check @mkConₚ
-
--- E
-#check @eConₛ
-#check @eConₚ
-
--- G
-#check @gConₛ
-#check @gConₚ
-#check GConₛA
-#check GConₚA
-
-#print axioms mkConₛ
-#print axioms mkConₚ
 
 structure Ind where
   Γₛ : Q(Conₛ.{0})
