Reflection/Derive.lean
@@ -7,8 +7,9 @@ open Reflection MutualInductive
 
 namespace Reflection.MutualInductive.Derive
 
-private partial def getTyₛ (tys : Expr) : MetaM Q(Tyₛ.{u}) := do
-  forallBoundedTelescope tys (some 1) fun var body => do
+/-- Reads in `Nat -> Type`. -/
+partial def getTyₛ (τ : Q(Type (u+1))) : MetaM Q(Tyₛ.{u}) := do
+  forallBoundedTelescope τ (some 1) fun var body => do
     if var.isEmpty then
       return q(Tyₛ.U.{u})
     else
@@ -17,6 +18,143 @@ private partial def getTyₛ (tys : Expr) : MetaM Q(Tyₛ.{u}) := do
       let rest : Q(Tyₛ.{u}) <- getTyₛ body -- rest is for example `var : X ⊢ SPi ...`
       let rest : Q($ty -> Tyₛ.{u}) <- mkLambdaFVars #[var] rest
       return q(Tyₛ.SPi.{u} $ty $rest)
+
+set_option pp.universes true in
+#print Nₛ
+#eval getTyₛ (u := .zero) q(Type)
+#eval getTyₛ (u := .zero) q(Nat -> Type)
+
+def _root_.List.indexOf [BEq α] : List α -> α -> Option Nat
+| []     , _ => none
+| x :: xs, a => if x == a then some 0 else (indexOf xs a).map (. + 1)
+
+partial def Conₛ.recMeta {motive : Q(Type u)} (Γₛ : Q(Conₛ.{u}))
+  (case_nil : MetaM Q($motive))
+  (case_ext : Q(Conₛ.{u}) -> MetaM Q($motive) -> Q(Tyₛ.{u}) -> MetaM Q($motive))
+  : MetaM Q($motive)
+  := do
+    let Γₛ : Q(Conₛ.{u}) <- whnf Γₛ
+    match Γₛ with
+    | ~q(Conₛ.nil.{u}) => case_nil
+    | ~q(Conₛ.ext.{u} $Δₛ $Bₛ) => case_ext Δₛ (Conₛ.recMeta Δₛ case_nil case_ext) Bₛ
+    | _ => throwError "Conₛ.recMeta: nonexhaustive match, have Γₛ ≣ q({Γₛ})"
+
+-- #check Tyₛ.SPi
+-- #check Tyₛ.rec
+-- /-
+-- {motive : Tyₛ → Sort u_1} →
+--   motive Tyₛ.U →
+--   ((T : Type u) → (a : T → Tyₛ) →    ((a_1 : T) → motive (a a_1))    → motive (Tyₛ.SPi T a))
+--   → (t : Tyₛ) → motive t
+-- -/
+-- partial def Tyₛ.recMeta {motive : Q(Type u)} (Aₛ : Q(Tyₛ.{u}))
+--   (case_U : MetaM Q($motive))
+--   (case_SPi : (T : Q(Type u)) -> Q($T -> Tyₛ.{u}) -> Q($T -> $motive) -> MetaM Q($motive))
+--   : MetaM Q($motive)
+--   := do
+--     match Aₛ with
+--     | ~q(Tyₛ.U.{u}) => case_U
+--     | ~q(Tyₛ.SPi.{u} $T $f) => case_SPi T f (<- Tyₛ.recMeta )
+
+def getVarₛ (n : Nat) (Γₛ : Q(Conₛ.{u})) (Aₛ : Q(Tyₛ.{u})) : MetaM Q(Varₛ.{u} $Γₛ $Aₛ) := do
+  Conₛ.recMeta Γₛ
+    (throwError "getVarₛ: Γₛ is nil")
+    (fun Δₛ _ih Bₛ => do
+      match n with
+      | 0 =>
+        let .true <- isDefEq Bₛ Aₛ | throwError "getVarₛ n=0: isDefEq failed: {Aₛ} is not defeq to {Bₛ}"
+        return mkApp2 q(@Varₛ.vz.{u}) Δₛ Bₛ
+      | n + 1 =>
+        let var : Q(Varₛ $Δₛ $Aₛ) <- getVarₛ n Δₛ Aₛ
+        return .app q(@Varₛ.vs $Δₛ $Aₛ $Bₛ) var
+    )
+
+def ctx : Q(Conₛ.{0}) := q((⬝ ▹ Tyₛ.U) ▹ Tyₛ.U)
+#eval getVarₛ (u := 0) 0 ctx q(Tyₛ.U)
+#eval getVarₛ (u := 0) 1 ctx q(Tyₛ.U)
+
+#check @Tmₛ.app
+
+/-- Reads in `Vec 123`. Make sure that `mblock` has the names of `Γₛ` in the same order. -/
+partial def getTmₛ (mblock : List Name) (Γₛ : Q(Conₛ.{u})) (Aₛ : Q(Tyₛ.{u})) (T : Q(TyₛA.{u, u} $Aₛ)) : MetaM Q(Tmₛ.{u} $Γₛ $Aₛ) := do
+  match T with
+  | .const name _ =>
+    let some idx := mblock.indexOf name | throwError "getTmₛ case Tyₛ.U: {T} does not belong to mutual block {mblock}"
+    let var <- getVarₛ idx Γₛ Aₛ
+    return q(Tmₛ.var $var)
+  | .app f x => -- case `Vec 123 : TyₛA Aₛ`
+    let ⟨u', ⟨X, x⟩⟩ <- inferTypeQ x -- x : X
+    unless <- isLevelDefEq (.succ u) u' do throwError "getTmₛ level defeq failed, u ≣ {u}, but u' ≣ {u'}, with X ≣ {X}"
+    -- let fTy <- inferType f
+    let Bₛ : Q($X -> Tyₛ.{u}) <- mkFreshExprMVarQ q($X -> Tyₛ.{u})
+    let fTy <- inferType f -- q(Nat -> Type)
+    let fTy_code : Q(Tyₛ.{u}) <- getTyₛ (u := u) fTy -- q("Nat -> Type")
+    let fTy_code_A : Q(Type (u+1)) := q(TyₛA.{u,u} $fTy_code) -- q("Nat -> Type"ᴬ) ≣ q((x : $X) -> "$Bₛ x"ᴬ)
+    -- let fTy_expected := q((x : $X) -> TyₛA.{u,u} ($Bₛ x))
+    unless <- isDefEq fTy_code_A q((x : $X) -> TyₛA.{u,u} ($Bₛ x)) do
+      throwError "getTmₛ defeq type of f to function type failed, f : {<- inferType f}, X ≣ {X}, x ≣ {x}, Bₛ ≣ {Bₛ}\nfTy ≣ {()}\nfTy_code ≣ asdf"
+    throwError "stop\nfTy ≣ {fTy}\nfTy_code ≣ {fTy_code}\nfTy_code_A ≣ {fTy_code_A}\nfTy_code_A₂ ≣ {q((x : $X) -> TyₛA.{u,u} ($Bₛ x))}"
+
+
+    let f : Q((x : $X) -> TyₛA.{u,u} ($Bₛ x)) := f -- can do this because of the defeq check
+    let f : Q(TyₛA.{u,u} ($Bₛ $x)) := f -- can do this because of the defeq check
+
+    let sub <- getTmₛ mblock Γₛ fTy_code q($f)
+    return mkAppN q(Tmₛ.app.{u}) #[] --#[Γₛ, X, Bₛ, f, x]
+  | _ => throwError "oh no, getTmₛ {T}"
+
+#check Vₛ
+inductive Vec : Nat -> Type
+#eval getTmₛ (u := .zero) [``Nat] q(Nₛ) q(.U) q(Nat)
+#eval getTmₛ (u := .zero) [``Nat] q(Nₛ) q(.U) q(Nat) >>= inferType
+#eval getTmₛ (u := .zero) [``Vec] q(Vₛ) q(.U) q(Vec 123)
+-- #eval getTmₛ (u := .zero) [``Vec] q(Vₛ) q(.U) q(Vec 123)
+
+#exit
+
+/-- Parse a constructor type, for example `(n : Nat) -> Even n -> Odd (n+1)`. -/
+partial def getTyₚ (mblock : List Name) (Γₛ : Q(Conₛ.{u})) (tys : Expr) : MetaM Q(Tyₚ.{u} $Γₛ) := do
+  forallBoundedTelescope tys (some 1) fun var body => do
+    if var.isEmpty then -- `El T`
+      let T <- getTmₛ Γₛ q(Tyₛ.U.{u}) body
+      return q(Tyₚ.El.{u} $T)
+    else -- PFunc or PPi
+      let var := var[0]!
+      let ty : Q(Type u) <- var.fvarId!.getType
+      let .const tyF _ := ty.getAppFn | throwError "getTyₚ parameter {ty}"
+      if mblock.contains tyF then -- PFunc
+        let T : Q(Tmₛ.{u} $Γₛ Tyₛ.U) <- getTmₛ Γₛ q(Tyₛ.U.{u}) ty
+        let rest <- getTyₚ mblock Γₛ body
+        return q(Tyₚ.PFunc.{u} $T $rest)
+      else -- PPi
+        let rest : Q($ty -> Tyₚ.{u} $Γₛ) <- getTyₚ mblock Γₛ body
+        return q(Tyₚ.PPi.{u} $ty $rest)
+
+partial def getConₛ (block : InductiveVal) : MetaM Q(Conₛ.{u}) := do
+  block.all.foldlM (fun (acc : Q(Conₛ.{u})) I => do
+    let info <- getConstInfoInduct I
+    let ty : Q(Tyₛ.{u}) <- getTyₛ info.type
+    return q(Conₛ.ext $acc $ty)
+  ) q(Conₛ.nil.{u})
+
+partial def getConₚ (block : InductiveVal) (Γₛ : Q(Conₛ.{u})) : MetaM Q(Conₚ.{u} $Γₛ) := do
+  let allCtors : List Name <- block.all.foldlM (fun (acc : List Name) I => do
+    let info <- getConstInfoInduct I
+    return info.ctors ++ acc
+  ) []
+  allCtors.foldlM (fun (acc : Q(Conₚ.{u} $Γₛ)) c => do
+    let info <- getConstInfoCtor c
+    let ty <- getTyₚ block.all Γₛ info.type
+    return q(Conₚ.ext $acc $ty)
+  ) q(Conₚ.nil.{u})
+
+elab "getConₛ! " i:ident : term => do
+  let ind <- getConstInfoInduct i.getId
+  let u <- mkFreshLevelMVar
+  getConₛ (u := u) ind
+
+#check Vec
+#check getConₛ! Vec
 
 partial def skipParams (tys : Expr) (nParams : Nat) (cont : Expr -> MetaM Expr) : MetaM Expr :=
   match nParams with
@@ -27,12 +165,12 @@ partial def skipParams (tys : Expr) (nParams : Nat) (cont : Expr -> MetaM Expr) 
       if body'.containsFVar var[0]!.fvarId! then mkLambdaFVars var body'
       else return body'
 
-elab "Tyₛ% " tys:term : term => do
+elab "getTyₛ! " tys:term : term => do
   let tys <- elabTerm tys none
   let u <- mkFreshLevelMVar
   getTyₛ (u:=u) tys
 
-elab "Tyₛ! " T:term : term => do
+elab "Tyₛ% " T:term : term => do
   let T <- elabTerm T none
   let ⟨I, args⟩ := T.getAppFnArgs
   let info <- getConstInfoInduct I
@@ -40,22 +178,39 @@ elab "Tyₛ! " T:term : term => do
   let u <- mkFreshLevelMVar
   skipParams info.type info.numParams (getTyₛ (u := u))
 
-elab "Conₛ! " T:term : term => do
+elab "Conₛ% " T:term : term => do
   let T <- elabTerm T none
   let ⟨I, args⟩ := T.getAppFnArgs
   let info <- getConstInfoInduct I
   if info.numParams != args.size then throwError m!"Expected {info.numParams} params."
   let u <- mkFreshLevelMVar
-  info.all.foldlM (fun (acc : Q(Conₛ.{u})) name => do
-    let info <- getConstInfoInduct name
-    let u <- mkFreshLevelMVar
-    let ty : Q(Tyₛ.{u}) <- skipParams info.type info.numParams (getTyₛ (u := u))
-    return q(Conₛ.ext $acc $ty)
-  ) q(Conₛ.nil.{u})
+  getConₛ (u := u) info
 
-#check Tyₛ% (Nat -> Type)
-#check Tyₛ! (Vec String)
-#check Conₛ! (Vec String)
+elab "Conₚ% " T:term : term => do
+  let T <- elabTerm T none
+  let ⟨I, args⟩ := T.getAppFnArgs
+  let info <- getConstInfoInduct I
+  if info.numParams != args.size then throwError m!"Expected {info.numParams} params."
+  let u <- mkFreshLevelMVar
+  getConₛ (u := u) info
+
+elab "%Tyₚ " i:ident : term => do
+  let ind <- getConstInfoInduct i.getId
+  getTyₚ ind.all
+
+mutual
+  inductive Even : Nat -> Type
+  | zero : Even 0
+  | even : Odd n -> Even (n+1)
+  inductive Odd : Nat -> Type
+  | odd : Even n -> Odd (n+1)
+end
+
+#check getTyₛ! (Nat -> Type)
+#check Tyₛ% (Vec String)
+#check Conₛ% (Vec String)
+#check Conₛ% (Even)
+-- example
 
 -- /-- Given a `T` such as `Vec 123 : Type`, produce `Tmₛ.app (Tmₛ.var Varₛ.vz) 123 : Tmₛ _ Tyₛ.U`.
 --   Given `Vec : Nat -> Type`, produce `Tmₛ.var Varₛ.vz : Tmₛ _ (Tyₛ.SPi Nat fun _ => Tyₛ.U)`. -/
@@ -74,29 +229,6 @@ elab "Conₛ! " T:term : term => do
 --   -- let  := T.getAppFn
 --   let ind <- getConstInfoInduct (getAppFn)
 --   getTyₚ ind.type
-
-partial def getTyₚ (Γₛ : Q(Conₛ.{u})) (tys : Expr) : MetaM Q(Tyₚ.{u} $Γₛ) := do
-  forallBoundedTelescope tys (some 1) fun var body => do
-    if var.isEmpty then
-      return q(Tyₛ.U.{u})
-    else
-      let var := var[0]!
-      let ty : Q(Type u) <- var.fvarId!.getType
-      let rest : Q(Tyₛ.{u}) <- getTyₛ body -- rest is for example `var : X ⊢ SPi ...`
-      let rest : Q($ty -> Tyₛ.{u}) <- mkLambdaFVars #[var] rest
-      return q(Tyₛ.SPi.{u} $ty $rest)
-  -- forallBoundedTelescope args (some 1) fun var body => do
-  --   let u <- mkFreshLevelMVar
-  --   if var.isEmpty then
-  --     -- body is e.g. `Vec 123`.
-  --     let T <- getTmₛ Γₛ q(Tyₛ.U) body
-  --     return q(Tyₚ.El $(T))
-  --   else
-  --     let var := var[0]!
-  --     let ty : Q(Type u) <- var.fvarId!.getType
-  --     let rest : Expr <- getTyₛ body -- rest is for example `var : X ⊢ SPi ...`
-  --     let rest : Q($ty -> Tyₛ.{u}) <- mkLambdaFVars #[var] rest -- rest is for example `⊢ fun var:X => SPi ...`
-  --     return q(Tyₛ.SPi.{u} $ty $rest)
 
 elab "%Tyₚ " i:ident : term => do
   let ind <- getConstInfoInduct i.getId
