lakefile.lean
@@ -9,6 +9,7 @@ require std from git "https://github.com/leanprover/std4" @ "nightly-testing-202
 require aesop from git "https://github.com/JLimperg/aesop" @ "5fefb40a7c9038a7150e7edd92e43b1b94c49e79"
 -- require IIT from git "https://github.com/arthur-adjedj/iit" @ "v4.4.0"
 require Qq from git "https://github.com/leanprover-community/quote4"
+-- require mathlib from git "https://github.com/leanprover-community/mathlib4"
 
 @[default_target]
 lean_lib «Reflection» {
